Snapshot: trigger anomaly in Coq (issue: it appears that you cannot do type-class search when defining cofixpoints?)

src/threadpool/trace.v
@@ -5,104 +5,280 @@ From Paco Require Import paco.
 From Paco Require Import paco2.
 From stdpp Require Import list.
 
-Definition scheduler {E R} : itree (threadpoolE +' E) R → list (itree (threadpoolE +' E) R) → itree E (R + last_thread_killed) :=
-  cofix _scheduler t tp :=
+Section scheduler.
+  Definition scheduler {E R} : itree (threadpoolE +' E) R → list (itree (threadpoolE +' E) R) → itree E (R + last_thread_killed) :=
+    cofix _scheduler t tp :=
+        match observe t with
+        | RetF r  => Ret (inl r)
+        | TauF t' => Tau (_scheduler t' tp)
+        | @VisF _ _ _ A (inl1 e) k =>
+          (match e with
+          | EFork => λ k, Tau (_scheduler (k CurrentThread) (k NewThread :: tp))
+          | EYield => λ k, Tau (_scheduler (k ()) tp)
+          | EKillThread => λ k,
+              match tp with
+              | [] => Ret (inr LastThreadKilled)
+              | t' :: tp' => Tau (_scheduler t' tp')
+              end
+          end : (A → _) → _) k
+        | VisF (inr1 e) k => Vis e (λ a, _scheduler (k a) tp)
+        end.
+  Notation scheduler_ t tp :=
       match observe t with
       | RetF r  => Ret (inl r)
-      | TauF t' => Tau (_scheduler t' tp)
+      | TauF t' => Tau (scheduler t' tp)
       | @VisF _ _ _ A (inl1 e) k =>
         (match e with
-        | EFork => λ k, Tau (_scheduler (k CurrentThread) (k NewThread :: tp))
-        | EYield => λ k, Tau (_scheduler (k ()) tp)
+        | EFork => λ k, Tau (scheduler (k CurrentThread) (k NewThread :: tp))
+        | EYield => λ k, Tau (scheduler (k ()) tp)
         | EKillThread => λ k,
             match tp with
             | [] => Ret (inr LastThreadKilled)
-            | t' :: tp' => Tau (_scheduler t' tp')
+            | t' :: tp' => Tau (scheduler t' tp')
             end
         end : (A → _) → _) k
-      | VisF (inr1 e) k => Vis e (λ a, _scheduler (k a) tp)
+      | VisF (inr1 e) k => Vis e (λ a, scheduler (k a) tp)
       end.
-Notation scheduler_ t tp :=
-    match observe t with
-    | RetF r  => Ret (inl r)
-    | TauF t' => Tau (scheduler t' tp)
-    | @VisF _ _ _ A (inl1 e) k =>
-      (match e with
-      | EFork => λ k, Tau (scheduler (k CurrentThread) (k NewThread :: tp))
-      | EYield => λ k, Tau (scheduler (k ()) tp)
-      | EKillThread => λ k,
-          match tp with
-          | [] => Ret (inr LastThreadKilled)
-          | t' :: tp' => Tau (scheduler t' tp')
-          end
-      end : (A → _) → _) k
-    | VisF (inr1 e) k => Vis e (λ a, scheduler (k a) tp)
-    end.
 
-Lemma unfold_scheduler {E R} (t : itree (threadpoolE +' E) R) tp :
-  scheduler t tp = scheduler_ t tp.
-Proof.
-  apply bisimulation_is_eq. apply observing_sub_eqit; constructor; reflexivity.
+  Lemma unfold_scheduler {E R} (t : itree (threadpoolE +' E) R) tp :
+    scheduler t tp = scheduler_ t tp.
+  Proof.
+    apply bisimulation_is_eq. apply observing_sub_eqit; constructor; reflexivity.
+  Qed.
+
+  Lemma list_delete_insert {A} idx x (xs : list A) :
+    delete idx (<[idx := x]> xs) = delete idx xs.
+  Proof.
+    induction idx as [|idx IH] in xs |- *.
+    - destruct xs as [|x' xs']; done.
+    - destruct xs as [|x' xs'].
+      * done.
+      * simpl. f_equiv. apply IH.
+  Qed.
+
+  Lemma list_delete_empty {A} idx (xs : list A) :
+    delete idx xs = [] →
+    length xs <= 1.
+  Proof.
+    intros Hemp.
+    destruct (decide (idx < length xs)).
+    - replace (length xs) with (length (delete idx xs) + 1).
+      * rewrite Hemp //.
+      * rewrite length_delete. { lia. }
+        by apply lookup_lt_is_Some_2.
+    - rewrite delete_take_drop take_ge in Hemp.
+      * apply app_nil in Hemp as [-> _]. simpl. lia.
+      * lia.
+  Qed.
+
+  Lemma schedule_exists {E R} (t : itree (threadpoolE +' E) R) tid tp :
+    tp !! tid = Some t →
+    interleaves tid tp (scheduler t (delete tid tp)).
+  Proof.
+    intros Hidx.
+    remember (scheduler t (delete tid tp)) as t'.
+    revert t tp tid Hidx t' Heqt'. pcofix CIH. intros t tp tid Hidx t' ->.
+    pfold. exists t. split; first done.
+    rewrite unfold_scheduler.
+    destruct (observe t) as [r'|t'|A e k].
+    - constructor.
+    - constructor. right. apply (CIH t').
+      apply lookup_lt_Some in Hidx.
+      rewrite list_lookup_insert //.
+      rewrite list_delete_insert //.
+    - destruct e as [e|e]; first destruct e.
+      * constructor. right. apply (CIH (k CurrentThread)).
+        + simpl. apply lookup_lt_Some in Hidx.
+          rewrite list_lookup_insert; eauto.
+        + rewrite /= list_delete_insert //.
+      * apply Yield with (new_current_tid := tid). right.
+        apply (CIH (k ())).
+        + simpl. apply lookup_lt_Some in Hidx.
+          rewrite list_lookup_insert; eauto.
+        + rewrite /= list_delete_insert //.
+      * apply singleton_or_more in Hidx as [[-> ->]|[Hlen Hidx]].
+        + constructor.
+        + destruct (delete tid tp) as [|t' tp'] eqn:Heq.
+          ++ apply list_delete_empty in Heq. lia.
+          ++ apply KillThread with (new_current_tid := 0).
+             right. apply CIH with (t := t'); rewrite Heq //.
+      * constructor. intros a. right.
+        apply CIH with (t := k a).
+        + rewrite list_lookup_insert //. by apply lookup_lt_is_Some.
+        + by rewrite list_delete_insert.
+  Qed.
+End scheduler.
+
+CoInductive ctrace (E : Type → Type) (R : Type) :=
+  | CTRet (r : R)
+  | CTVis (A : Type) (e : E A) (a : A) (k : ctrace E R)
+  | CTTau (k : ctrace E R)
+  | CTYield (new_tid : nat) (k : ctrace E R)
+  | CTKillThread (new_tid : nat) (k : ctrace E R)
+  | CTKillLastThread
+  | CTFork (t : itree (threadpoolE +' E) R) (k : ctrace E R)
+  | CTCut.
+
+Arguments CTRet {_ _}.
+Arguments CTVis {_ _}.
+Arguments CTTau {_ _}.
+Arguments CTYield {_ _}.
+Arguments CTKillThread {_ _}.
+Arguments CTKillLastThread {_ _}.
+Arguments CTFork {_ _}.
+Arguments CTCut {_ _}.
+
+CoInductive trace (E : Type → Type) (R : Type) :=
+  | TRet (r : R)
+  | TVis (A : Type) (e : E A) (a : A) (k : trace E R)
+  | TTau (k : trace E R)
+  | TCut.
+
+Class AnswerEqDecision (E : Type → Type) :=
+  is_AnswerEqDecision A : E A → EqDecision A.
+Print RelDecision.
+Print Decision.
+
+Program Definition equal `{AnswerEqDecision E} {A : Type} (e : E A) (a a' : A) : {a = a'} + {a ≠ a'} :=
+  @decide (a = a') _.
+Next Obligation.
+  intros E Hdec A e a a'. by apply is_AnswerEqDecision.
 Qed.
 
-Lemma list_delete_insert {A} idx x (xs : list A) :
-  delete idx (<[idx := x]> xs) = delete idx xs.
-Proof.
-  induction idx as [|idx IH] in xs |- *.
-  - destruct xs as [|x' xs']; done.
-  - destruct xs as [|x' xs'].
-    * done.
-    * simpl. f_equiv. apply IH.
-Qed.
+Section extend_ctrace.
+  Context {E : Type → Type} {R : Type} `{AnswerEqDecision E}.
 
-Lemma list_delete_empty {A} idx (xs : list A) :
-  delete idx xs = [] →
-  length xs <= 1.
-Proof.
-  intros Hemp.
-  destruct (decide (idx < length xs)).
-  - replace (length xs) with (length (delete idx xs) + 1).
-    * rewrite Hemp //.
-    * rewrite length_delete. { lia. }
-      by apply lookup_lt_is_Some_2.
-  - rewrite delete_take_drop take_ge in Hemp.
-    * apply app_nil in Hemp as [-> _]. simpl. lia.
-    * lia.
-Qed.
+  Definition extend_ctrace_to_interleaving_ : ctrace E R → nat → itree (threadpoolE +' E) R → list (itree (threadpoolE +' E) R) → itree E (R + last_thread_killed) :=
+    cofix _extend_ctrace_to_interleaving tr tid t tp :=
+        match tr with
+        | CTRet r => Ret (inl r)
+        | CTVis A e a tr' => Vis e (λ a', if equal e a a' then _extend_ctrace_to_interleaving tr' tid t tp else scheduler t (delete tid tp))
+        | CTTau tr' => Tau (_extend_ctrace_to_interleaving tr' tid t tp)
+        | CTYield new_tid tr' =>
+            match tp !! new_tid with
+            | Some t' => Tau (_extend_ctrace_to_interleaving tr' new_tid t' tp)
+            (* Placeholder: should never happen. *)
+            | None => ITree.spin
+            end
+        | _ => Ret (inr LastThreadKilled)
+        end.
 
-Lemma schedule_exists {E R} (t : itree (threadpoolE +' E) R) tid tp :
-  tp !! tid = Some t →
-  interleaves tid tp (scheduler t (delete tid tp)).
-Proof.
-  intros Hidx.
-  remember (scheduler t (delete tid tp)) as t'.
-  revert t tp tid Hidx t' Heqt'. pcofix CIH. intros t tp tid Hidx t' ->.
-  pfold. exists t. split; first done.
-  rewrite unfold_scheduler.
-  destruct (observe t) as [r'|t'|A e k].
-  - constructor.
-  - constructor. right. apply (CIH t').
-    apply lookup_lt_Some in Hidx.
-    rewrite list_lookup_insert //.
-    rewrite list_delete_insert //.
-  - destruct e as [e|e]; first destruct e.
-    * constructor. right. apply (CIH (k CurrentThread)).
-      + simpl. apply lookup_lt_Some in Hidx.
-        rewrite list_lookup_insert; eauto.
-      + rewrite /= list_delete_insert //.
-    * apply Yield with (new_current_tid := tid). right.
-      apply (CIH (k ())).
-      + simpl. apply lookup_lt_Some in Hidx.
-        rewrite list_lookup_insert; eauto.
-      + rewrite /= list_delete_insert //.
-    * apply singleton_or_more in Hidx as [[-> ->]|[Hlen Hidx]].
-      + constructor.
-      + destruct (delete tid tp) as [|t' tp'] eqn:Heq.
-        ++ apply list_delete_empty in Heq. lia.
-        ++ apply KillThread with (new_current_tid := 0).
-           right. apply CIH with (t := t'); rewrite Heq //.
-    * constructor. intros a. right.
-      apply CIH with (t := k a).
-      + rewrite list_lookup_insert //. by apply lookup_lt_is_Some.
-      + by rewrite list_delete_insert.
-Qed.
+        | TauF t' => Tau (_scheduler t' tp)
+        | @VisF _ _ _ A (inl1 e) k =>
+          (match e with
+          | EFork => λ k, Tau (_scheduler (k CurrentThread) (k NewThread :: tp))
+          | EYield => λ k, Tau (_scheduler (k ()) tp)
+          | EKillThread => λ k,
+              match tp with
+              | [] => Ret (inr LastThreadKilled)
+              | t' :: tp' => Tau (_scheduler t' tp')
+              end
+          end : (A → _) → _) k
+        | VisF (inr1 e) k => Vis e (λ a, _scheduler (k a) tp)
+        end.
+  Notation scheduler_ t tp :=
+      match observe t with
+      | RetF r  => Ret (inl r)
+      | TauF t' => Tau (scheduler t' tp)
+      | @VisF _ _ _ A (inl1 e) k =>
+        (match e with
+        | EFork => λ k, Tau (scheduler (k CurrentThread) (k NewThread :: tp))
+        | EYield => λ k, Tau (scheduler (k ()) tp)
+        | EKillThread => λ k,
+            match tp with
+            | [] => Ret (inr LastThreadKilled)
+            | t' :: tp' => Tau (scheduler t' tp')
+            end
+        end : (A → _) → _) k
+      | VisF (inr1 e) k => Vis e (λ a, scheduler (k a) tp)
+      end.
+
+  Lemma unfold_scheduler {E R} (t : itree (threadpoolE +' E) R) tp :
+    scheduler t tp = scheduler_ t tp.
+  Proof.
+    apply bisimulation_is_eq. apply observing_sub_eqit; constructor; reflexivity.
+  Qed.
+
+extend_ctrace_to_interleaving :: ctrace → ITree (threadpoolE +' E) R → ITree E R
+is_ctrace :: ctrace → ITree (threadpoolE +' E) R → Prop
+is_trace :: trace → ITree E R → Prop
+tracify :: ctrace → trace
+
+Lemma :
+  is_ctrace ctr t →
+  interleaving t (extend_ctrace_to_interleaving ctr t).
+Lemma :
+  is_ctrace ctr t →
+  is_trace (tracify ctr) (extend_ctrace_to_interleaving ctr t).
+
+
+Section traced_interleaving.
+  Context {E : Type → Type} {R : Type}.
+
+  Variant traced_interleavesF
+    (traced_interleaves : trace E R → nat → list (itree (threadpoolE +' E) R) → itree E (R + last_thread_killed) → Prop)
+    : trace E R
+    → nat
+    → itree' (threadpoolE +' E) R
+    → list (itree (threadpoolE +' E) R)
+    → itree' E (R + last_thread_killed)
+    → Prop :=
+  | Return current_tid tp r :
+    traced_interleavesF interleaves (TRet r) current_tid (RetF r) tp (RetF (inl r))
+  | Step trace' current_tid current' tp interleaving' :
+    traced_interleaves current_tid trace' (<[current_tid:=current']>tp) interleaving' →
+    traced_interleavesF interleaves (TTau trace') current_tid (TauF current') tp (TauF interleaving')
+  | Emit trace' current_tid tp A (e : E A) a k k' :
+    (∀ a, interleaves current_tid (<[current_tid:=k a]>tp) (k' a)) →
+    traced_interleavesF interleaves trace' current_tid (<[current_tid:=k a]>tp) (k' a) →
+    traced_interleavesF interleaves (TVis A e a trace') current_tid (VisF (inr1 e) k) tp (VisF e k')
+  | KillThread trace' current_tid tp k new_current_tid interleaving' :
+    traced_interleaves trace' new_current_tid (delete current_tid tp) interleaving' →
+    traced_interleavesF interleaves (TKillThread new_current_tid trace') current_tid (VisF (inl1 EKillThread) k) tp (TauF interleaving')
+  | KillLastThread k t :
+    traced_interleavesF interleaves TKillLastThread 0 (VisF (inl1 EKillThread) k) [t] (RetF (inr LastThreadKilled))
+  | Yield trace' current_tid tp k new_current_tid interleaving' :
+    traced_interleaves trace' new_current_tid (<[current_tid := k ()]>tp) interleaving' →
+    traced_interleavesF interleaves (TYield new_current_tid trace') current_tid (VisF (inl1 EYield) k) tp (TauF interleaving')
+  | Fork trace' current_tid tp k interleaving' :
+    traced_interleaves (S current_tid) (k NewThread :: <[current_tid := k CurrentThread]>tp) interleaving' →
+    traced_interleavesF interleaves (TFork (k CurrentThread) trace') current_tid (VisF (inl1 EFork) k) tp (TauF interleaving').
+  (* TODO: Somehow deal with the case where the main thread emits
+  [EKillThread]. (This case is never exhibited for typical [itree]s, because
+  [EKillThread] is generally only to be used to avoid forked threads from
+  returning.) For example, return an [option]. *)
+  Hint Constructors interleavesF : iris_itree.
+  (** The recuirsion template for the interleaving relation. *)
+  Definition interleaves_
+    (interleaves : nat → list (itree (threadpoolE +' E) R) → itree E (R + last_thread_killed) → Prop)
+    : nat
+    → list (itree (threadpoolE +' E) R)
+    → itree E (R + last_thread_killed)
+    → Prop :=
+    λ tid tp interleaving, ∃ t, tp !! tid = Some t ∧ interleavesF interleaves tid (observe t) tp (observe interleaving).
+
+  Lemma interleavesF_mono interleaves interleaves' tid t tp interleaving :
+    interleaves <3= interleaves' →
+    interleavesF interleaves tid t tp interleaving →
+    interleavesF interleaves' tid t tp interleaving.
+  Proof.
+    intros Hleq HinterleavesF. destruct HinterleavesF; eauto with iris_itree.
+  Qed.
+  Lemma interleaves__mono :
+    monotone3 interleaves_.
+  Proof.
+    rewrite /monotone3 /interleaves_. intros tid tp t r r' [t' [Hidx Hinter]] Hrel.
+    eexists. split; first done. by eapply interleavesF_mono; last done.
+  Qed.
+  Hint Resolve interleaves__mono : paco.
+
+  (** The interleaving relation. (See comments above.) *)
+  Definition interleaves : nat → list (itree (threadpoolE +' E) R) → itree E (R + last_thread_killed) → Prop :=
+    paco3 interleaves_ bot3.
+
+  Lemma interleaves_lookup tid tp interleaving :
+    interleaves tid tp interleaving →
+    ∃ t, tp !! tid = Some t.
+  Proof.
+    intros Hinter. punfold Hinter. destruct Hinter as [t' [Hidx' Hinter]]. eauto.
+  Qed.
